theories/Semantics.v
@@ -2,24 +2,32 @@ From Stdlib Require Import Utf8.
 
 From Stdlib Require Import Lists.List.
 From Stdlib Require Import ZArith.ZArith.
-From Stdlib Require Import Relations.Relations.
+
+From stdpp Require Import gmap.
+From stdpp Require Import relations.
 
 From RSL Require Import Tactics.
-From RSL Require Import NatMap.
 From RSL Require Import RTL.
 From RSL Require Import Notations.
 
 Import RTLNotations.
 Import ListNotations.
 
+(* Set Mangle Names. *)
+
 (* [regmap] is a mapping from registers to a value *)
-Definition regmap : Type := NatMap.t val.
+Definition regmap : Type := gmap reg val.
 
 (* [memory] is a mapping from location to a value *)
-Definition memory : Type := NatMap.t val.
+Definition memory : Type := gmap loc val.
+
+Definition val_to_loc (v: val) : option loc :=
+  if (v >=? 1)%Z
+  then Some (Z.to_pos v)
+  else None.
 
 Definition get_reg (ρ: regmap) (r: reg) : val :=
-  match NatMap.find r ρ with
+  match ρ !! r with
   | Some v => v
   | None => 0%Z (* Dummy val *)
   end.
@@ -27,26 +35,30 @@ Definition get_reg (ρ: regmap) (r: reg) : val :=
 Definition get_regs (ρ: regmap) (l: list reg) : list val :=
   map (fun r => get_reg ρ r) l.
 
-Definition set_reg (ρ: regmap) (r: reg) (v: val) : regmap :=
-  NatMap.add r v ρ.
+Definition set_reg (ρ: regmap) (r: reg) (v: val) : regmap := <[r := v]>ρ.
 
 Definition get_at (m: memory) (addr: val) : option val :=
-  if (addr >=? 0)%Z
-  then NatMap.find (Z.to_nat addr) m
-  else None.
+  match val_to_loc addr with
+  | Some loc => m !! loc
+  | None => None
+  end.
+
+Definition update_at (m: memory) (addr: val) (f: val -> val) : option memory
+  := match val_to_loc addr with
+     | Some loc =>
+         match m !! loc with
+         | Some old => Some (<[loc := f old]>m)
+         | None => None
+         end
+     | None => None
+     end.
 
 Definition set_at (m: memory) (addr: val) (v: val) : option memory :=
-  if (addr >=? 0)%Z
-  then
-    let addr := Z.to_nat addr in
-    if NatMap.mem addr m
-    then Some (NatMap.add addr v m)
-    else None
-  else None.
+  update_at m addr (fun _ => v).
 
 (* Assert that instruction at [pc] in function [f] is [i] *)
 Notation "f '@' pc 'is' i" :=
-  (NatMap.find pc (fn_code f) = Some i) (at level 60, no associativity).
+  ((fn_code f)!!pc = Some i) (at level 60, no associativity).
 
 Definition eval_op (op: op) (args: list val) : option val :=
   match op, args with
@@ -60,8 +72,8 @@ Definition eval_op (op: op) (args: list val) : option val :=
 
 Fixpoint init_regs (vl: list val) (rl: list reg) : regmap :=
   match rl, vl with
-  | r :: rs, v :: vs => NatMap.add r v (init_regs vs rs)
-  | _, _ => NatMap.empty _
+  | r :: rs, v :: vs => <[r := v]>(init_regs vs rs)
+  | _, _ => ∅
   end.
 
 Inductive stackframe : Type :=
@@ -88,101 +100,100 @@ Inductive pcstate : Type :=
 
 Definition state : Type := list stackframe * pcstate * memory.
 
-Definition find_fun (P: program) (s: sig) : option function :=
-  List.find
-    (fun f =>
-       let sig := fn_sig f in
-       let same_len :=
-         Nat.eqb (List.length (in_regs sig)) (List.length (in_regs s)) in
-       let same_name := String.eqb (name sig) (name s) in
-       andb same_len same_name) P.
-
-Reserved Notation "P '⊢' s '->>' t" (at level 60, right associativity).
+Reserved Notation "P '|-' s '->>' t" (at level 60, right associativity).
 
 Inductive step (P: program) : state -> state -> Prop :=
 | exec_Inop: forall σ m ρ f pc pc',
   f@pc is <{ nop -> pc' }> ->
-  P ⊢ (σ, State f pc ρ, m) ->> (σ, State f pc' ρ, m)
+  P |- (σ, State f pc ρ, m) ->> (σ, State f pc' ρ, m)
 
 | exec_Iret: forall σ m ρ f pc r v,
   f@pc is <{ ret r }> ->
   get_reg ρ r = v ->
-  P ⊢ (σ, State f pc ρ, m) ->> (σ, ReturnState v, m)
+  P |- (σ, State f pc ρ, m) ->> (σ, ReturnState v, m)
 
 | exec_Iop: forall σ m ρ f pc op args dst pc' ρ' v,
   f@pc is <{ dst := @op args -> pc' }> ->
   eval_op op (get_regs ρ args) = Some v ->
   set_reg ρ dst v = ρ' ->
-  P ⊢ (σ, State f pc ρ, m) ->> (σ, State f pc' ρ', m)
+  P |- (σ, State f pc ρ, m) ->> (σ, State f pc' ρ', m)
 
 | exec_Iload: forall σ m ρ f pc dst src pc' ρ' addr v,
   f@pc is <{ dst := !src -> pc' }> ->
   get_reg ρ src = addr ->
   get_at m addr = Some v ->
   set_reg ρ dst v = ρ' ->
-  P ⊢ (σ, State f pc ρ, m) ->> (σ, State f pc' ρ', m)
+  P |- (σ, State f pc ρ, m) ->> (σ, State f pc' ρ', m)
 
 | exec_Istore: forall σ m ρ f pc dst src pc' m' addr v,
   f@pc is <{ !dst := src -> pc' }> ->
   get_reg ρ dst = addr ->
   get_reg ρ src = v ->
   set_at m addr v = Some m' ->
-  P ⊢ (σ, State f pc ρ, m) ->> (σ, State f pc' ρ, m')
+  P |- (σ, State f pc ρ, m) ->> (σ, State f pc' ρ, m')
 
 | exec_Icond: forall  σ m ρ f pc cond ifso ifnot v pc',
   f@pc is <{ if cond then goto ifso else goto ifnot }> ->
   get_reg ρ cond = v ->
   pc' = (if Z.eqb v 0 then ifso else ifnot) ->
-  P ⊢ (σ, State f pc ρ, m) ->> (σ, State f pc' ρ, m)
+  P |- (σ, State f pc ρ, m) ->> (σ, State f pc' ρ, m)
 
 | exec_Icall: forall σ m ρ f pc dst sig args pc' σ' fn,
   f@pc is <{ dst := @call sig args -> pc' }> ->
   find_fun P sig = Some fn ->
   Stackframe dst f pc' ρ :: σ = σ' ->
-  P ⊢ (σ, State f pc ρ, m) ->> (σ', CallState fn (get_regs ρ args), m)
+  P |- (σ, State f pc ρ, m) ->> (σ', CallState fn (get_regs ρ args), m)
 
 | exec_function: forall σ m ρ f args,
   init_regs args (in_regs f.(fn_sig)) = ρ ->
-  P ⊢ (σ, CallState f args, m) ->> (σ, State f (fn_entrypoint f) ρ, m)
+  P |- (σ, CallState f args, m) ->> (σ, State f (fn_entrypoint f) ρ, m)
 
 | exec_return: forall σ m ρ f pc dst v ρ',
   set_reg ρ dst v = ρ' ->
-  P ⊢ (Stackframe dst f pc ρ :: σ, ReturnState v, m) ->> (σ, State f pc ρ', m)
+  P |- (Stackframe dst f pc ρ :: σ, ReturnState v, m) ->> (σ, State f pc ρ', m)
 
-where "P '⊢' s '->>' t" := (step P s t).
+where "P '|-' s '->>' t" := (step P s t).
 
-Definition steps (P: program) : state -> state -> Prop
-  := clos_refl_trans state (step P).
+Notation "P '|-' s '->>*' t" :=
+  (rtc (step P) s t)  (at level 60, right associativity).
 
-Notation "P '⊢' s '->>*' t" :=
-  (steps P s t) (at level 60, right associativity).
+Notation "P '|-' s '-{' n '}>' t" :=
+  (nsteps (step P) n s t)  (at level 60, right associativity).
 
-#[global]
-Add Parametric Relation (P: program) : state (steps P)
-  reflexivity proved by (rt_refl state (step P))
-  transitivity proved by (rt_trans state (step P))
-  as steps_rel.
+Lemma nsteps_inv_l {A : Type} {R : relation A} :
+  ∀ n x z, nsteps R (S n) x z → ∃ y : A, R x y ∧ nsteps R n y z.
+Proof. intros n x z H; inv H; eexists; eauto. Qed.
 
-Lemma inv_step : forall P s t,
-  P ⊢ s ->>* t -> s = t ∨ ∃ s', P ⊢ s ->> s' ∧ P ⊢ s' ->>* t.
+Lemma ret_no_step P : ∀ v m t,
+  P |- ([], ReturnState v, m) ->>* t ->
+  t = ([], ReturnState v, m).
 Proof.
-  intros P s t Hred.
-  apply clos_rt_rt1n_iff in Hred.
-  destruct Hred as [ | s' t H Hred ].
-  - auto.
-  - apply clos_rt_rt1n_iff in Hred. right. now exists s'.
+  intros v m t H.
+  destruct (rtc_inv _ _ H) as [-> | (y & Hstep & _)].
+  - easy.
+  - inv Hstep.
+Qed.
+
+Lemma ret_no_nsteps P : ∀ n v m t,
+  P |- ([], ReturnState v, m) -{n}> t ->
+  t = ([], ReturnState v, m) ∧ n = 0.
+Proof.
+  intros [] v m t H.
+  - now inv H.
+  - destruct (nsteps_inv_l _ _ _ H) as (y & Hstep & _).
+    inv Hstep.
 Qed.
 
 Lemma lift_step P : ∀ σ s m σ' t m' Σ,
-  P ⊢ (σ, s, m) ->> (σ', t, m') ->
-  P ⊢ (σ ++ Σ, s, m) ->> (σ' ++ Σ, t, m').
+  P |- (σ, s, m) ->> (σ', t, m') ->
+  P |- (σ ++ Σ, s, m) ->> (σ' ++ Σ, t, m').
 Proof.
   intros ? ? ? ? ? ? ? H; inv H; econstructor; now eauto.
 Qed.
 
 Lemma unlift_step P : ∀ σ s m σ' t m' Σ,
-  P ⊢ (σ ++ Σ, s, m) ->> (σ' ++ Σ, t, m') ->
-  P ⊢ (σ, s, m) ->> (σ', t, m').
+  P |- (σ ++ Σ, s, m) ->> (σ' ++ Σ, t, m') ->
+  P |- (σ, s, m) ->> (σ', t, m').
 Proof.
   intros ? ? ? ? ? ? ? H; inv H;
     rewrite ? app_comm_cons in *;
@@ -191,64 +202,58 @@ Proof.
 Qed.
 
 Theorem step_callstack P : ∀ σ s m σ' t m' Σ,
-  P ⊢ (σ, s, m) ->> (σ', t, m') <->
-  P ⊢ (σ ++ Σ, s, m) ->> (σ' ++ Σ, t, m').
+  P |- (σ, s, m) ->> (σ', t, m') <->
+  P |- (σ ++ Σ, s, m) ->> (σ' ++ Σ, t, m').
 Proof. split. 1: apply lift_step. apply unlift_step. Qed.
 
 Theorem lift_steps P : ∀ σ s m σ' t m' Σ,
-  P ⊢ (σ, s, m) ->>* (σ', t, m') ->
-  P ⊢ (σ ++ Σ, s, m) ->>* (σ' ++ Σ, t, m').
+  P |- (σ, s, m) ->>* (σ', t, m') ->
+  P |- (σ ++ Σ, s, m) ->>* (σ' ++ Σ, t, m').
 Proof.
-  intros σ s m σ' t m' Σ Hred.
+  intros σ s m σ' t m' Σ Hrtc.
   remember (σ, s, m) as x eqn:Hx.
   remember (σ', t, m') as y eqn:Hy.
-  revert σ s m Hx σ' t m' Hy.
-  apply clos_rt_rt1n_iff in Hred.
-  induction Hred as [ y | x y z Hstep Hred IH ].
-  - intros ? ? ? -> ? ? ? H. inv H. reflexivity.
-  - intros ? ? ? -> ? ? ? H. destruct y as [[] ?].
+  induction Hrtc as [ y | x y z H Hrtc IH]
+    in σ, s, m, Hx, σ', t, m', Hy |- *.
+  - subst. inv Hy. reflexivity.
+  - subst. destruct y as [[] ?].
     etransitivity.
-    + apply rt_step; apply lift_step; eassumption.
+    + apply rtc_once. apply lift_step. eassumption.
     + eauto.
 Qed.
 
-Lemma unfold_call P fn : ∀ res f pc ρ args m σ t m',
-  P ⊢ ([Stackframe res f pc ρ], CallState fn args, m) ->>* (σ, t, m') ->
+Lemma unfold_call P fn : ∀ n res f pc ρ args m σ t m',
+  P |- ([Stackframe res f pc ρ], CallState fn args, m) -{n}> (σ, t, m') ->
   (∃ σ',
       σ = σ' ++ [Stackframe res f pc ρ]
-      ∧ P ⊢ ([], CallState fn args, m) ->>* (σ', t, m'))
+      ∧ P |- ([], CallState fn args, m) -{n}> (σ', t, m'))
   ∨
-    (∃ v m'',
-        P ⊢ ([], CallState fn args, m) ->>* ([], ReturnState v, m'')
-        ∧ P ⊢ ([], State f pc (set_reg ρ res v), m'') ->>* (σ, t, m')
+    (∃ m1 m2 v m'',
+        n = 1 + m1 + m2
+        ∧ P |- ([], CallState fn args, m) -{m1}> ([], ReturnState v, m'')
+        ∧ P |- ([], State f pc (set_reg ρ res v), m'') -{m2}> (σ, t, m')
     ).
 Proof.
-  intros res f pc ρ args m σ t m' H.
-  remember [Stackframe res f pc ρ] as l.
-  remember (l, CallState fn args, m) as s1 eqn:Hs1.
-  remember (σ, t, m') as s2 eqn:Hs2.
-  revert s2 H σ t m' Hs2.
-  induction 1 as [ | [[σ1 t1] m1] z Hred IH Hstep]
-                   using clos_refl_trans_ind_left;
-    intros σ t m' ->.
-  - inv Hs1. left. now exists [].
-  - destruct (IH _ _ _ (eq_refl _ )) as
-      [(σ' & -> & Hlift) | (v & m'' & Hcall & Hrest)]; clear IH.
+  intros n.
+  induction n as [ | n IH ];
+    intros res f pc ρ args m σ t m' Hrtc.
+  - inv Hrtc. left. exists []. split; auto. constructor.
+  - apply nsteps_inv_r in Hrtc. destruct Hrtc as ([[] ?] & Hrtc & Hstep).
+    apply IH in Hrtc.
+    destruct Hrtc
+      as [(σ' & -> & Hlift) | (m1 & m2 & v & m'' & Hn & Hcall & Hrest)].
     + inv Hstep;
         try (left; eexists; split;
              [ rewrite ? app_comm_cons; reflexivity
-             | eapply rt_trans; [ apply Hlift | apply rt_step];
-               econstructor; now eauto
+             | eapply nsteps_r; [ now apply Hlift | econstructor; now eauto]
              ]
           ).
       destruct σ'; inv H.
-      * right. repeat eexists; now eauto.
+      * right. exists n, 0, v, m'. repeat split; eauto. constructor.
       * left. eexists. split.
         -- reflexivity.
-        -- eapply rt_trans; [apply Hlift | apply rt_step];
-             econstructor; now eauto.
-    + inversion Hstep; subst; right; repeat eexists;
-        now eauto ||
-          (eapply rt_trans; [apply Hrest | apply rt_step];
-           econstructor; now eauto).
+        -- eapply nsteps_r; [ now apply Hlift | econstructor; now eauto].
+    + inversion Hstep; subst; right; (exists m1, (S m2), v, m''); repeat split;
+        now eauto || (eapply nsteps_r;
+                      [ now apply Hrest | econstructor; now eauto]).
 Qed.
