theories/WP.v
@@ -4,12 +4,13 @@ From Stdlib Require Import Lists.List.
 From Stdlib Require Import Strings.String.
 From Stdlib Require Import ZArith.ZArith.
 From Stdlib Require Import Lia.
-From Stdlib Require Import Relations.Relations.
 
-From RSL Require Import NatMap.
+From stdpp Require Import relations.
+
 From RSL Require Import RTL.
 From RSL Require Import Notations.
 From RSL Require Import Semantics.
+From RSL Require Import Logic.
 From RSL Require Import Tactics.
 
 Import RTLNotations.
@@ -20,110 +21,180 @@ Import ListNotations.
 Section WP.
   Variable P : program.
 
-  Definition postcondition : Type := val -> memory -> Prop.
-
   Inductive final (Q: postcondition) : state -> Prop :=
   | Final : ∀ v m, Q v m -> final Q ([], ReturnState v, m).
 
-  Definition safe (Q: postcondition) (s: state) : Prop :=
-    ∀ t, P ⊢ s ->>* t -> final Q t ∨ ∃ u, P ⊢ t ->> u.
+  Definition not_stuck t := ∃ u, P |- t ->> u.
 
-  Definition wp (f: function) (pc: node) (Q: postcondition)
-    : regmap * memory -> Prop :=
-    fun '(ρ, m) => safe Q ([], State f pc ρ, m).
+  Lemma ret_not_stuck : ∀ frame σ v m,
+    not_stuck (frame :: σ, ReturnState v, m).
+  Proof. intros []. repeat econstructor; now eauto. Qed.
 
-  Lemma wp_ret f pc Q : forall v,
-    f@pc is <{ ret v }> ->
-    ∀ ρ m, Q (get_reg ρ v) m -> wp f pc Q (ρ, m).
+  Lemma ret_stuck_in_empty : ∀ v m,
+    ~ not_stuck ([], ReturnState v, m).
+  Proof. intros v m [u H]. inv H. Qed.
+
+  Lemma lift_not_stuck : ∀ σ Σ s m,
+    not_stuck (σ, s, m) ->
+    not_stuck (σ ++ Σ, s, m).
+  Proof. intros σ Σ s m [[[] ?] Ht]. eexists. apply lift_step. eassumption. Qed.
+
+  (** [safeₙ Q n s] : s is a state that is safe for at most n steps:
+      - s is a final step or
+      - s is not stuck and can do at most n steps. *)
+  Inductive safeₙ (Q : postcondition) : state -> nat -> Prop :=
+  | safe_init : ∀ s, safeₙ Q s 0
+  | final_is_safe : ∀ s, final Q s -> ∀ n, safeₙ Q s n
+  | safe_to_step : ∀ s n,
+    (* I am not stuck *)
+    not_stuck s ->
+    (* All possible next states are safe for at most n least *)
+    (∀ t, P |- s ->> t -> safeₙ Q t n) ->
+    (* I am safe for at most n+1 least *)
+    safeₙ Q s (S n).
+
+  Lemma safe_weakening Q s n :
+    ∀ m,
+    m <= n ->
+    safeₙ Q s n ->
+    safeₙ Q s m.
   Proof.
-    intros v H ρ m.
-    unfold wp, safe.
-    intros Hwp t Hred.
-    destruct (inv_step _ _ _ Hred) as [ <- | (ss & Hreds & Hrtc )].
-    - right. eexists. econstructor; now eauto.
-    - inv Hreds; try congruence.
-      destruct (inv_step _ _ _ Hrtc) as [ <- | (? & Hwhat & ? )].
-      + pc_inj. left. constructor. assumption.
-      + inversion Hwhat.
+    intros m Hle Hsafe.
+    induction Hsafe as [s' | s' Hfin n' | s' n' Hns Hstep IH] in m, Hle |- *.
+    - inv Hle. constructor.
+    - now constructor.
+    - destruct m as [ |m].
+      + constructor.
+      + apply safe_to_step; auto.
+        intros t Ht.
+        apply IH; auto.
+        lia.
+  Qed.
+
+  Lemma safe_from_progress Q s n :
+    (∀ t m,
+       m <= n ->
+       P |- s -{m}> t ->
+       final Q t ∨ not_stuck t)
+    -> safeₙ Q s n.
+  Proof.
+    intros H.
+    induction n as [ |n IH] in s, H |- *.
+    - apply safe_init.
+    - assert (Hstep: P |- s -{0}> s) by constructor.
+      assert (Hle: 0 <= S n) by lia.
+      destruct (H s 0 Hle Hstep) as [Hfin | Hns];
+        clear Hstep Hle.
+      + now constructor.
+      + apply safe_to_step; auto. intros t Hstep.
+        apply IH. intros u m Hle Hsteps.
+        apply (H u (S m)).
+        -- lia.
+        -- econstructor; now eauto.
+  Qed.
+
+  Lemma safe_implies_progress Q s n :
+    safeₙ Q s n ->
+    ∀ m t, m < n ->
+           P |- s -{m}> t ->
+           final Q t ∨ not_stuck t.
+  Proof.
+    intros Hsafe.
+    induction Hsafe as [s' | s' Hfin n' | s' n' Hns Hsafe IH];
+      intros m t Hlt Hrtc.
+    - inv Hlt.
+    - destruct m.
+      + inv Hrtc. auto.
+      + apply nsteps_inv_l in Hrtc. destruct Hrtc as (? & H & ?).
+        inv Hfin. inv H.
+    - destruct m.
+      + inv Hrtc. auto.
+      + apply nsteps_inv_l in Hrtc.
+        destruct Hrtc as (u & Hstep & Hrtc).
+        eapply IH; eauto. lia.
+  Qed.
+
+  Definition safe Q s := ∀ n, safeₙ Q s n.
+
+  Definition wp__n Q f pc : sProp :=
+    fun n '(ρ, m) => safeₙ Q ([], State f pc ρ, m) n.
+
+  Lemma wp_ret f pc Q : ∀ v,
+    f@pc is <{ ret v }> ->
+    (λₛ ρ m, ⌜Q (get_reg ρ v) m⌝) ⊢ wp__n Q f pc.
+  Proof.
+    intros v H [] [ρ m] HQ; [apply safe_init | ].
+    apply safe_to_step.
+    - eexists; econstructor; now eauto.
+    - intros t Hstep. inv Hstep. apply final_is_safe. now constructor.
   Qed.
 
   Lemma wp_nop f pc Q : forall pc',
     f@pc is <{ nop -> pc' }> ->
-    ∀ ρ m, wp f pc' Q (ρ, m) -> wp f pc Q (ρ, m).
+    ▷ wp__n Q f pc' ⊢ wp__n Q f pc.
   Proof.
-    intros pc' H ρ m.
-    unfold wp, safe.
-    intros Hwp t Hred.
-    destruct (inv_step _ _ _ Hred) as [ <- | (ss & Hreds & Hrtc )].
-    - right. eexists. econstructor; now eauto.
-    - apply Hwp; inv Hreds; pc_inj; congruence.
+    intros v H [] [ρ m] Hwp; [apply safe_init | ].
+    apply safe_to_step.
+    - repeat econstructor; now eauto.
+    - intros ? Hs. now inv Hs.
   Qed.
 
   Lemma wp_op f pc Q : forall dst op args pc',
     f@pc is <{ dst := @op args -> pc' }> ->
-    ∀ ρ m,
-    (∃ v,
-        eval_op op (get_regs ρ args) = Some v
-        ∧ wp f pc' Q (set_reg ρ dst v, m)
-    ) -> wp f pc Q (ρ, m).
+    ▷ (λₛ ρ m,
+         ∃ v,
+           ⌜eval_op op (get_regs ρ args) = Some v⌝
+           ∧ wp__n Q f pc' ⟨ set_reg ρ dst v, m ⟩
+    ) ⊢ wp__n Q f pc.
   Proof.
-    intros dst op args pc' H ρ m.
-    unfold wp, safe.
-    intros (v & Hv & Hwp) t Hred.
-    destruct (inv_step _ _ _ Hred) as [ <- | (ss & Hreds & Hrtc )].
-    - right. eexists. econstructor; now eauto.
-    - apply Hwp; inv Hreds; pc_inj; congruence.
+    intros dst op args pc' H [] [ρ m] Hwp; [apply safe_init | ].
+    destruct Hwp as (v & Hv & Hwp). unfold_sProp.
+    apply safe_to_step.
+    - repeat econstructor; now eauto.
+    - intros ? Hs. now inv Hs.
   Qed.
 
   Lemma wp_load f pc Q : forall dst src pc',
     f@pc is <{ dst := !src -> pc' }> ->
-    ∀ ρ m,
-    (
-      let addr := get_reg ρ src in
-      ∃ v, get_at m addr = Some v ∧  wp f pc' Q (set_reg ρ dst v, m)
-    ) -> wp f pc Q (ρ, m).
+    ▷ (λₛ ρ m,
+         let addr := get_reg ρ src in
+         ∃ v, ⌜get_at m addr = Some v⌝
+              ∧ wp__n Q f pc' ⟨ set_reg ρ dst v, m ⟩
+    ) ⊢ wp__n Q f pc.
   Proof.
-    intros dst src pc' H ρ m.
-    unfold wp, safe.
-    intros (v & Hv & Hwp) t Hred.
-    destruct (inv_step _ _ _ Hred) as [ <- | (ss & Hreds & Hrtc )].
-    - right. eexists. econstructor; now eauto.
-    - apply Hwp; inv Hreds; pc_inj; try congruence.
+    intros dst src pc' H [] [ρ m] Hwp; [apply safe_init | ].
+    destruct Hwp as (v & Hv & Hwp). unfold_sProp.
+    apply safe_to_step.
+    - repeat econstructor; now eauto.
+    - intros ? Hs. now inv Hs.
   Qed.
 
   Lemma wp_store f pc Q : forall dst src pc',
     f@pc is <{ !dst := src -> pc' }> ->
-    ∀ ρ m,
-    (
-      let addr := get_reg ρ dst in
-      let v := get_reg ρ src in
-      ∃ m', set_at m addr v = Some m' ∧ wp f pc' Q (ρ, m')
-    ) -> wp f pc Q (ρ, m).
+    ▷ (λₛ ρ m,
+         let addr := get_reg ρ dst in
+         let v := get_reg ρ src in
+         ∃ m', ⌜set_at m addr v = Some m'⌝
+               ∧ wp__n Q f pc' ⟨ ρ, m' ⟩
+    ) ⊢ wp__n Q f pc.
   Proof.
-    intros dst src pc' H ρ m.
-    unfold wp, safe.
-    intros (v & Hv & Hwp) t Hred.
-    destruct (inv_step _ _ _ Hred) as [ <- | (ss & Hreds & Hrtc )].
-    - right. eexists. econstructor; now eauto.
-    - apply Hwp; inv Hreds; pc_inj; congruence.
+    intros dst src pc' H [] [ρ m] Hwp; [apply safe_init | ].
+    destruct Hwp as (v & Hv & Hwp). unfold_sProp.
+    apply safe_to_step.
+    - repeat econstructor; now eauto.
+    - intros ? Hs. now inv Hs.
   Qed.
 
   Lemma wp_cond f pc Q : forall cond ifso ifnot,
     f@pc is <{ if cond then goto ifso else goto ifnot }> ->
-    ∀ ρ m,
-    (
-      if (get_reg ρ cond =? 0)%Z
-      then wp f ifso Q (ρ, m)
-      else wp f ifnot Q (ρ, m)
-    ) -> wp f pc Q (ρ, m).
+    ▷ (λₛ ρ m,
+         wp__n Q f (if (get_reg ρ cond =? 0)%Z then ifso else ifnot)
+      ) ⊢ wp__n Q f pc.
   Proof.
-    intros cond ifso ifnot H ρ m.
-    unfold wp, safe.
-    intros Hwp t Hred.
-    destruct (inv_step _ _ _ Hred) as [ <- | (ss & Hreds & Hrtc)].
-    - right. eexists. econstructor; now eauto.
-    - inv Hreds; pc_inj; try congruence.
-      destruct (get_reg ρ cond =? 0)%Z eqn:Hcond; auto.
+    intros cond ifso ifnot H [] [ρ m] Hwp; [apply safe_init | ].
+    unfold_sProp. apply safe_to_step.
+    - repeat econstructor; now eauto.
+    - intros ? Hs. now inv Hs.
   Qed.
 
   Definition precondition : Type := list val -> memory -> Prop.
@@ -134,98 +205,56 @@ Section WP.
   Notation "'{{' P '}}' f '{{' Q '}}'" :=
     (hoare P f Q) (at level 90, f at next level).
 
+  Lemma hoare_post_from_steps Pre f Post :
+    {{ Pre }} f {{ Post }} ->
+    ∀ n args m v m',
+    P |- ([], CallState f args, m) -{n}> ([], ReturnState v, m') ->
+    Pre args m ->
+    Post v m'.
+  Proof.
+    intros Hspec n args m v m' Hsteps Hpre.
+    eapply safe_implies_progress with (n := S n) in Hsteps.
+    - destruct Hsteps as [Hfin | Hstuck].
+      + inv Hfin. eassumption.
+      + apply ret_stuck_in_empty in Hstuck. tauto.
+    - now apply Hspec.
+    - lia.
+  Qed.
+
   Lemma wp_call f pc Q : ∀ dst sig args pc',
     f@pc is <{ dst := @call sig args -> pc' }> ->
-    ∀ ρ m,
-    (∃ fn Pre Post,
-        let vals := get_regs ρ args in
-        find_fun P sig = Some fn ∧
-        {{ Pre }} fn {{ Post }} ∧
-        Pre vals m ∧
-        ∀ v m', let ρ' := set_reg ρ dst v in
-                Post v m' -> wp f pc' Q (ρ', m')
-    ) -> wp f pc Q (ρ, m).
+    ▷ (λₛ ρ m,
+         ∃ fn Pre Post,
+           let vals := get_regs ρ args in
+           ⌜find_fun P sig = Some fn⌝ ∧
+           ⌜{{ Pre }} fn {{ Post }}⌝ ∧
+           ⌜Pre vals m⌝ ∧
+           ∀ v m', ⌜Post v m'⌝ -> wp__n Q f pc' ⟨ set_reg ρ dst v, m' ⟩
+      ) ⊢ wp__n Q f pc.
   Proof.
-    intros dst sig args pc' H ρ m.
-    unfold wp, safe.
-    intros (fn & Pre & Post & Hfun & Hspec & Hpre & Hwp) t Hred.
-    destruct (inv_step _ _ _ Hred) as [ <- | (ss & Hreds & Hrtc)].
-    - right. eexists. econstructor; now eauto.
-    - inv Hreds; pc_inj; try congruence. pc_inj.
-      destruct t as [[σ' s] m''] eqn:Ht.
-      destruct (unfold_call _ _ _ _ _ _ _ _ _ _  _ Hrtc)
-        as [(σ'' & Hσ & Hrtc') | (v & m' & Hrtc' & Hrest)].
-      + destruct (Hspec _ _ Hpre _ Hrtc') as [Hfin | (u & Hu)].
-        * inv Hfin; simpl. right. eexists. econstructor; now eauto.
-        * right. destruct u as [[]?]. subst.
-          eexists. apply lift_step. apply Hu.
-      + destruct (Hspec _ _ Hpre _ Hrtc') as [Hfin | (u & Hu)].
-        * inv Hfin; simpl. eapply Hwp; eassumption.
-        * inversion Hu.
+    intros dst sig args pc' H [ | n] [ρ m] Hwp; [apply safe_init | ].
+    destruct Hwp as (fn & Pre & Post & Hfun & Hspec & Hpre & Hwp).
+    unfold_sProp. apply safe_to_step.
+    - repeat econstructor; now eauto.
+    - intros t Hs. inv Hs.
+      apply safe_from_progress.
+      intros [[σ' s] m''] n' Hn Hsteps.
+      apply unfold_call in Hsteps.
+      destruct Hsteps as [(? & ? & Hrtc) | (? & ? & ? & ? & ? & Hrtc & Hrest)].
+      + right. pose proof (Hspec _ _ Hpre (S n)) as Hfunsafe.
+        edestruct (safe_implies_progress _ _ _ Hfunsafe n')
+          as [Hfin | Hprogress]; eauto with lia.
+        * inv Hfin. apply ret_not_stuck.
+        * subst. now apply lift_not_stuck.
+      + eapply safe_implies_progress in Hrest.
+        * eassumption.
+        * apply Hwp.
+          apply (hoare_post_from_steps _ _ _ Hspec) in Hrtc; auto.
+        * lia.
   Qed.
 End WP.
 
-Section WP2.
-  Variable P : program.
-  (* Definition stuck s := ~ (∃ t, P ⊢ s ->> t) ∧ ~ (final s). *)
-
-  (* Definition not_stuck s := final s ∨ ∃ t, P ⊢ s ->> t. *)
-
-  Fixpoint wp2_ (n: nat) (s: state) (Q: postcondition) :=
-    match n with
-    | O => True
-    | S n =>
-        (final Q s) ∨ ((∃ t, P ⊢ s ->> t) ∧ ∀ t, P ⊢ s ->> t -> wp2_ n t Q)
-    end.
-
-  Definition wp2 (s: state) (Q: postcondition) := ∀ n, wp2_ n s Q.
-
-  Lemma safe_to_wp2 : ∀ s Q,
-    safe P Q s -> wp2 s Q.
-  Proof.
-    intros s Q H n. induction n as [ | n IH] in H, s |- *.
-    - easy.
-    - simpl. destruct (H s (rt_refl _ _ _)) as [Hfin | [t Ht]].
-      + auto.
-      + right. split.
-        * exists t. assumption.
-        * intros u Hu. apply IH. intros v Hv. apply H.
-          eapply rt_trans.
-          -- constructor. eassumption.
-          -- assumption.
-  Qed.
-
-  Lemma wp2_acc : ∀ s t Q,
-    P ⊢ s ->>* t ->
-    wp2 s Q ->
-    wp2 t Q.
-  Proof.
-    intros s t Q Hst.
-    induction Hst as [ s t H | s | s t u Hs IHs Ht IHt]; intros Hw.
-    - intros n. specialize (Hw (S n)). simpl in Hw.
-      destruct Hw as [Hfin | [_ Hall]].
-      + inversion Hfin; subst. inversion H.
-      + apply Hall. exact H.
-    - exact Hw.
-    - apply IHt. apply IHs. exact Hw.
-  Qed.
-
-  Lemma wp2_to_safe : ∀ s Q,
-    wp2 s Q -> safe P Q s.
-  Proof.
-    intros s Q Hwp. unfold wp2, safe.
-    intros t Hred.
-    apply (wp2_acc _ _ Q) in Hred; try assumption.
-    specialize (Hred 1). simpl in Hred.
-    destruct Hred as [?| [ ]]; auto.
-  Qed.
-
-  Theorem wp2_is_safe :
-    ∀ s Q, wp2 s Q <-> safe P Q s.
-  Proof.
-    intros s Q. split.
-    - apply wp2_to_safe.
-    - apply safe_to_wp2.
-  Qed.
-End WP2.
-
+(* Lemma wp_truc f pc Q : *)
+(*   ▷ ((∀ l ∈ L, ∀ ρ m, wp f l Q (ρ, m)) -> ∀ l ∈ L, ∀ ρ m, wp f l Q (ρ, m)) *)
+(*   ->∀ pc ∈ L,∀ ρ m, -> wp f pc Q (ρ, m). *)
+(* Proof. *)
