theories/Iris.v
@@ -1,2 +1,0 @@
-(* From iris.base_logic.lib Require Import gen_heap. *)
-
