theories/Logic.v
@@ -1,0 +1,149 @@
+From Stdlib Require Import Utf8.
+
+From RSL Require Import RTL.
+From RSL Require Import Semantics.
+
+Definition postcondition : Type := val -> memory -> Prop.
+Definition sProp : Type := nat -> regmap * memory -> Prop.
+
+Declare Scope sProp_scope.
+Delimit Scope sProp_scope with sProp.
+Bind Scope sProp_scope with sProp.
+
+Definition sProp_and (P Q : sProp) : sProp :=
+  fun n p => P n p ∧ Q n p.
+
+Notation "P ∧ Q" :=
+  (sProp_and P Q) : sProp_scope.
+
+Definition sProp_or (P Q : sProp) : sProp :=
+  fun n p => P n p ∨ Q n p.
+
+Notation "P ∨ Q" :=
+  (sProp_or P Q) : sProp_scope.
+
+Definition sProp_impl (P Q : sProp) : sProp :=
+  fun n p => P n p -> Q n p.
+
+Notation "P -> Q" :=
+  (sProp_impl P Q) : sProp_scope.
+
+Definition sProp_not (P : sProp) : sProp :=
+  fun n p => ~ P n p.
+
+Notation "~ P" :=
+  (sProp_not P) : sProp_scope.
+
+Definition sProp_exists {A : Type} (f : A -> sProp) : sProp :=
+  fun n p => ∃ x : A, f x n p.
+
+Notation "'∃' x .. y , p" :=
+  (sProp_exists (fun x => .. (sProp_exists (fun y => p)) ..)) : sProp_scope.
+
+Definition sProp_forall {A : Type} (f : A -> sProp) : sProp :=
+  fun n p => ∀ x : A, f x n p.
+
+Notation "'∀' x .. y , p" :=
+  (sProp_forall (fun x => .. (sProp_forall (fun y => p)) ..)) : sProp_scope.
+
+Definition sProp_pure (P : Prop) : sProp :=
+  fun _ _ => P.
+
+Notation "⌜ P ⌝" :=
+  (sProp_pure P)
+    (at level 0, format "⌜ P ⌝") : sProp_scope.
+
+Definition sProp_later (P : sProp) : sProp :=
+  fun n =>
+    match n with
+    | O => fun _ => True
+    | S n => fun p => P n p
+    end.
+
+Notation "▷ P" :=
+  (sProp_later P)
+    (at level 20, right associativity, format "▷ P") : sProp_scope.
+
+Definition sProp_always (P : sProp) : sProp :=
+  fun _ p => ∀ n, P n p.
+
+Notation "□ P" :=
+  (sProp_always P)
+    (at level 20, right associativity, format "□ P") : sProp_scope.
+
+Definition sProp_entails (P Q : sProp) : Prop :=
+  ∀ n p, P n p -> Q n p.
+
+Notation "P ⊢ Q" :=
+  (sProp_entails P%sProp Q%sProp)
+    (at level 99, right associativity).
+
+Definition sProp_ask (F : regmap -> memory -> sProp) : sProp :=
+  fun n '(ρ, m) => F ρ m n (ρ, m).
+
+Notation "'λₛ' ρ m , P" :=
+  (sProp_ask (fun ρ m => P))
+    (at level 200,
+        ρ name,
+        m name,
+        right associativity,
+        format "'λₛ' ρ  m  ,  P") : sProp_scope.
+
+Definition sProp_put (ρ : regmap) (m : memory) (P : sProp) : sProp :=
+  fun n _ => P n (ρ, m).
+
+Notation "P '⟨' ρ ',' m '⟩'" :=
+  (sProp_put ρ m P)
+    (at level 11,
+        left associativity,
+        format "P  '⟨' ρ ','  m '⟩'") : sProp_scope.
+
+Create HintDb custom_sProp discriminated.
+
+Hint Unfold
+  sProp_and
+  sProp_or
+  sProp_impl
+  sProp_not
+  sProp_exists
+  sProp_forall
+  sProp_pure
+  sProp_later
+  sProp_always
+  sProp_entails
+  sProp_ask
+  sProp_put
+: custom_sProp.
+
+Ltac unfold_sProp :=
+  autounfold with custom_sProp in *;
+  cbv beta in *;
+  simpl in *.
+
+Definition mono (P : sProp) : Prop :=
+  ∀ n p, P (S n) p -> P n p.
+
+Lemma later_intro S :
+  mono S -> S ⊢ ▷ S.
+Proof.
+  intros Hmono.
+  unfold_sProp.
+  intros [|n] p Hs.
+  - exact I.
+  - apply Hmono. exact Hs.
+Qed.
+
+Lemma löb S P :
+  mono S ->
+  (S ∧ ▷ P ⊢ P) -> S ⊢ P.
+Proof.
+  intros Hmono H n [ρ m] Hs.
+  induction n as [|n IHn].
+  - apply H. split.
+    + assumption.
+    + easy.
+  - apply H. split.
+    + assumption.
+    + apply IHn.
+      apply Hmono. assumption.
+Qed.
