theories/Tactics.v
@@ -1,11 +1,21 @@
 Ltac inv H := inversion H; subst; clear H.
 
+Ltac some_inj :=
+  match goal with
+  | [ H1: ?f = Some ?x, H2: ?f = Some ?y |- _ ] =>
+      let H := fresh in
+      assert (H: y = x) by congruence; subst; clear H2
+  end.
+
 Ltac pc_inj :=
   match goal with
   | [ H1: ?f = Some (?x1 ?x2), H2: ?f = Some (?y1 ?y2) |- _ ] =>
       let H := fresh in
       assert (H: y1 y2 = x1 x2) by congruence; inv H; clear H2
-  | [ H1: ?f = Some ?x, H2: ?f = Some ?y |- _ ] =>
-      let H := fresh in
-      assert (H: y = x) by congruence; subst; clear H2
+  end.
+
+Ltac case_if H :=
+  match type of H with
+  | if ?c then _ else _ =>
+      let H := fresh "HIfCond" in destruct c eqn:H
   end.
